src/pred_set/src/more_theories/permutesScript.sml
@@ -99,6 +99,12 @@ Proof
       PROVE_TAC [] ]
 QED
 
+Theorem permutes_bijn:
+  f permutes s <=> f IN bijns s
+Proof
+  simp[permutes_alt, bijns_def]
+QED
+
 Theorem permutes_alt_univ :
     !f. f permutes UNIV <=> f PERMUTES UNIV
 Proof
